Proof of the guts of lemma 2.10
This finally gets us over the line with the hard bits. We define it
with a "split map" (gluing together two functions depending on a
predicate) and then there's just a whole load of case analysis. Still
to do:

 - unpack the "smg_equiv" that we want in the lemma statement (rather
   than asking for the factorisations as an input)

 - Turn fin_subst into a sigma type to cut down on some of the
   argument passing.

Terms/Generality.v
@@ -1,6 +1,18 @@
-Require Import Top.Terms.Term.
-Require Import Top.Terms.Subst.
+Require Import Lists.List.
+Require Import Compare_dec.
+
+Require Import Top.FinSet.FinMod.
+Require Import Top.FinSet.FinSet.
+Require Import Top.FinSet.FPCard.
+Require Import Top.FinSet.NatMap.
+Require Import Top.FinSet.ProjSet.
+
+Require Import Top.Terms.BoundInImage.
 Require Import Top.Terms.FreeVars.
+Require Import Top.Terms.Perm.
+Require Import Top.Terms.SplitMap.
+Require Import Top.Terms.Subst.
+Require Import Top.Terms.Term.
 Require Import Top.Terms.VecUtils.
 
 (* First, we have to define the "more general than" relation on
@@ -52,6 +64,7 @@ Section smg.
 
 End smg.
 
+
 (** * Elements that are [sequiv] are related by a permutation
 
     This section is devoted to proving Lemma 2.10 from Eder's paper. This says
@@ -59,48 +72,22 @@ End smg.
     there are permutations that relabel them into each other.
 
 *)
-Section sequiv_means_perm.
+Section sequiv_means_perm_lt.
   Variable L : lType.
-  Variables sigma sigma' : Subst L.
-  Variables rho rho' : Subst L.
-  Hypothesis sigma'H : forall v, sigma' v = comp_subst L rho sigma v.
-  Hypothesis sigmaH : forall v, sigma v = comp_subst L rho' sigma' v.
+  Notation V := (Term.V L).
 
-  Lemma sigma_is_rho2_sigma v
-    : sigma v = comp_subst L (comp_subst L rho' rho) sigma v.
-  Proof.
-    rewrite <- comp_subst_assoc.
-    unfold comp_subst at 1; simpl.
-    rewrite <- sigma'H, sigmaH; auto.
-  Qed.
-
-  Lemma rho2_fixes_im_sigma v
-    : termset_fv v (subst_im L sigma) ->
-      comp_subst L rho' rho v = varTerm L v.
-  Proof.
-    apply (@comp_subst_determines_fvs
-             L sigma (comp_subst L rho' rho) (varTerm L)); clear v.
-    intro v; rewrite <- sigma_is_rho2_sigma, comp_subst_idl; auto.
-  Qed.
-
-  Lemma rho_im_sigma_has_height_0 v
-    : termset_fv v (subst_im L sigma) -> term_height (rho v) = 0.
-  Proof.
-    intro fvH.
-    apply PeanoNat.Nat.le_0_r.
-    apply (PeanoNat.Nat.le_trans _ _ _ (@term_height_comp_subst L rho' rho v)).
-    rewrite (rho2_fixes_im_sigma v fvH); auto.
-  Qed.
+  (** Firstly, we a helper function and facts about it. This function
+      takes a term of height zero (which must actually be a variable)
+      and extracts that variable. *)
 
   Definition unpack_height_0_term (t : Term L)
-    : term_height t = 0 -> Term.V L :=
+    : term_height t = 0 -> V :=
     match t with
     | varTerm _ v => fun _ => v
     | funTerm f ts =>
       fun htH =>
-        False_rect (Term.V L)
-                   (PeanoNat.Nat.neq_succ_0
-                      (vec_max_at (term_height (L:=L)) ts) htH)
+        False_rect _ (PeanoNat.Nat.neq_succ_0
+                        (vec_max_at (term_height (L:=L)) ts) htH)
     end.
 
   Lemma unpack_height_0_term_irrel
@@ -119,36 +106,134 @@ Section sequiv_means_perm.
     contradiction (PeanoNat.Nat.neq_succ_0 _ H).
   Qed.
 
-  Local Definition vrho
-             (v : Term.V L) (fvH : termset_fv v (subst_im L sigma)) : Term.V L :=
-    unpack_height_0_term (rho v) (rho_im_sigma_has_height_0 v fvH).
+  (** Now we throw in the assumptions used in lemma 2.10. Here, we
+      arbitrarily decide that there will be more bound variables in the
+      image of [sigma'] than in the image of [sigma]. We'll argue by
+      symmetry at the very end. *)
 
-  Lemma vrho_correct v (fvH : termset_fv v (subst_im L sigma))
-    : varTerm L (vrho v fvH) = rho v.
+  Variables sigma sigma' : Subst L.
+  Variables rho rho' : Subst L.
+  Hypothesis sigma'H : forall v, sigma' v = comp_subst L rho sigma v.
+  Hypothesis sigmaH : forall v, sigma v = comp_subst L rho' sigma' v.
+  Hypothesis finsigH : fin_subst L sigma.
+  Hypothesis finsig'H : fin_subst L sigma'.
+  Hypothesis finrhoH : fin_subst L rho.
+  Hypothesis decV : forall v v' : V, {v = v'} + {v <> v'}.
+
+  Definition biv_card_list (s : Subst L) (finH : fin_subst L s)
+    : fp_card_list (bound_image_var L s) :=
+    dec_fp_card_list (finite_bound_in_image L s finH decV) decV.
+
+  Definition biv_card (s : Subst L) (finH : fin_subst L s) : nat :=
+    fp_card (biv_card_list s finH).
+
+  Hypothesis cardleH : biv_card sigma finsigH <= biv_card sigma' finsig'H.
+
+  (** We are going to define the permutation by splitting [V] into
+      those variables that are free in the image of [sigma] and those
+      that are bound in the image of [sigma].
+
+      On the "free part", we will show that [rho] sends variables to
+      variables and we define [vrho] to get at these variables. *)
+
+  Lemma sigma_is_rho2_sigma v
+    : sigma v = comp_subst L (comp_subst L rho' rho) sigma v.
+  Proof.
+    rewrite <- comp_subst_assoc.
+    unfold comp_subst at 1; simpl.
+    rewrite <- sigma'H, sigmaH; auto.
+  Qed.
+
+  Definition is_sigma_fv (v : V) := termset_fv v (subst_im L sigma).
+  Definition is_sigma_bv (v : V) := is_bound_in_image L sigma v.
+
+  Definition fv_proj (x : sig is_sigma_fv) : V := proj1_sig x.
+  Definition bv_proj (x : sig is_sigma_bv) : V := proj1_sig x.
+
+  Lemma rho2_fixes_im_sigma v
+    : is_sigma_fv v -> comp_subst L rho' rho v = varTerm L v.
+  Proof.
+    apply (@comp_subst_determines_fvs
+             L sigma (comp_subst L rho' rho) (varTerm L)); clear v.
+    intro v; rewrite <- sigma_is_rho2_sigma, comp_subst_idl; auto.
+  Qed.
+
+  Lemma rho_im_sigma_has_height_0 v
+    : is_sigma_fv v -> term_height (rho v) = 0.
+  Proof.
+    intro fvH.
+    apply PeanoNat.Nat.le_0_r.
+    apply (PeanoNat.Nat.le_trans _ _ _ (@term_height_comp_subst L rho' rho v)).
+    rewrite (rho2_fixes_im_sigma v fvH); auto.
+  Qed.
+
+  Local Definition vrho (x : sig is_sigma_fv) : V :=
+    match x with
+    | exist _ v H =>
+      unpack_height_0_term (rho v) (rho_im_sigma_has_height_0 v H)
+    end.
+
+  Lemma vrho_correct v H
+    : varTerm L (vrho (exist _ v H)) = rho v.
   Proof.
     apply varTerm_unpack_height_0_term.
   Qed.
 
-  Lemma vrho_is_fv_for_sigma' v (fvH : termset_fv v (subst_im L sigma))
-    : termset_fv (vrho v fvH) (subst_im L sigma').
+  Lemma vrho_is_fv_for_sigma' x
+    : termset_fv (vrho x) (subst_im L sigma').
   Proof.
-    destruct fvH as [ t [ imH fvH' ] ].
+    destruct x as [ v fvH ]; destruct fvH as [ t [ imH fvH' ] ].
     generalize (ex_intro (fun t0 => _ /\ term_fv v t0) _
                          (conj imH fvH')); intro fvH.
     destruct imH as [ w tH ].
     rewrite tH in fvH'; clear t tH.
     rewrite termset_fv_subst_im; exists w.
     rewrite sigma'H.
-    apply (term_fv_in_subst_endo rho v (vrho v fvH) (sigma w) fvH').
+    apply (term_fv_in_subst_endo rho v _ (sigma w) fvH').
     rewrite <- (vrho_correct v fvH).
     simpl; auto.
   Qed.
 
-  Lemma vrho_irrel v (fvH0 fvH1 : termset_fv v (subst_im L sigma))
-    : vrho v fvH0 = vrho v fvH1.
+  Lemma vrho_irrel v (fvH0 fvH1 : is_sigma_fv v)
+    : vrho (exist _ v fvH0) = vrho (exist _ v fvH1).
   Proof.
-    unfold vrho.
-    auto using unpack_height_0_term_irrel.
+    unfold vrho; auto using unpack_height_0_term_irrel.
+  Qed.
+
+  (** We need to show some sort of finiteness property for [vrho]. The
+      obvious statement, [fin_mod fv_proj vrho] isn't true. The
+      problem is that the domain of [vrho] is itself a sigma type, so
+      you run into problems with how many proofs there are that a
+      given variable is free.
+
+      Instead of proving that, we "unpack" [fin_mod] slightly, and
+      construct a list of [mod_dom fv_proj vrho] elements (variables
+      free in the image of [sigma] for which [vrho] is not the
+      identity) where projecting all the way down to [V] does give a
+      [FullProj].
+
+      To do this, note that forgetting a variable is free gives an
+      injection from [mod_dom fv_proj vrho] into [mod_dom varTerm rho]
+      (variables for which [rho] is not [varTerm]). This forms a
+      commutative square with [id: V -> V] along the bottom and the
+      projection on the right is finite by finiteness of [rho].
+
+       All we need in order to use [finite_left_inverse] is to
+       construct a partial right inverse to this inclusion. *)
+
+  Definition dec_sigma_fv (v : V)
+    : {is_sigma_fv v} + {is_sigma_bv v} :=
+    dec_free_in_image L sigma decV _ (proj2_sig finsigH) v.
+
+  Lemma mod_elt_rho_to_vrho v
+        (neH : mod_elt (varTerm L) rho v)
+        (fvH : termset_fv v (subst_im L sigma))
+    : mod_elt fv_proj vrho (exist _ v fvH).
+  Proof.
+    unfold mod_elt, fv_proj, proj1_sig.
+    intro eqH; contradiction neH.
+    rewrite <- (f_equal (varTerm L) eqH).
+    rewrite vrho_correct; auto.
   Qed.
 
   Lemma varTerm_injective v w
@@ -157,19 +242,266 @@ Section sequiv_means_perm.
     injection 1; auto.
   Qed.
 
-  Lemma vrho_injective
-        v0 v1
-        (fv0H : termset_fv v0 (subst_im L sigma))
-        (fv1H : termset_fv v1 (subst_im L sigma))
-    : vrho v0 fv0H = vrho v1 fv1H ->
-      v0 = v1.
+  Lemma mod_elt_vrho_to_rho v
+        (fvH : termset_fv v (subst_im L sigma))
+        (neH : mod_elt fv_proj vrho (exist _ v fvH))
+    : mod_elt (varTerm L) rho v.
+  Proof.
+    unfold mod_elt, fv_proj, proj1_sig.
+    intro eqH; contradiction neH.
+    apply varTerm_injective.
+    rewrite vrho_correct; auto.
+  Qed.
+
+  Local Definition vrho_inj_top
+    : mod_dom fv_proj vrho -> mod_dom (varTerm L) rho :=
+    fun x =>
+      match x with
+      | exist _ (exist _ v fvH) neH => exist _ v (mod_elt_vrho_to_rho v fvH neH)
+      end.
+
+  Local Definition vrho_uninj_top
+    : mod_dom (varTerm L) rho -> option (mod_dom fv_proj vrho) :=
+    fun x =>
+      match x with
+      | exist _ v neH =>
+        match dec_sigma_fv v with
+        | left fvH => Some (exist _ (exist _ v fvH)
+                                  (mod_elt_rho_to_vrho v neH fvH))
+        | right bdH => None
+        end
+      end.
+
+  Local Definition vrho_uninj_bot : V -> option V :=
+    fun v =>
+      match dec_sigma_fv v with
+      | left fvH => Some v
+      | right bdH => None
+      end.
+
+  Lemma vrho_finite : FiniteProj (fun (x : mod_dom fv_proj vrho) =>
+                                    (fv_proj (md_elt x))).
+  Proof.
+    eapply (@finite_left_inverse (mod_dom fv_proj vrho)
+                                 (mod_dom (varTerm L) rho)
+                                 vrho_uninj_top
+                                 V V vrho_uninj_bot
+                                 (fun x => proj1_sig (md_elt x)) md_elt
+                                 _ vrho_inj_top id _ _ finrhoH).
+    Unshelve.
+    - intro x; destruct x as [ v neH ].
+      unfold vrho_uninj_top, vrho_uninj_bot; simpl.
+      destruct (dec_sigma_fv v); auto.
+    - intro x; destruct x as [ x neH ]; destruct x as [ v fvH ]; auto.
+    - intro x; destruct x as [ x neH ]; destruct x as [ v fvH ]; simpl.
+      unfold vrho_uninj_bot, id.
+      destruct (dec_sigma_fv v) as [ | bdH ]; [ auto | contradiction bdH ].
+  Qed.
+
+  Lemma vrho_injective x x'
+    : vrho x = vrho x' -> proj1_sig x = proj1_sig x'.
   Proof.
     intro vrhoH.
+    destruct x as [ v0 fv0H ], x' as [ v1 fv1H ]; simpl.
     apply varTerm_injective.
     rewrite <- (rho2_fixes_im_sigma v0 fv0H), <- (rho2_fixes_im_sigma v1 fv1H).
     unfold comp_subst; apply f_equal.
     rewrite <- (vrho_correct v0 fv0H), <- (vrho_correct v1 fv1H).
     apply f_equal, vrhoH.
+  Qed.
+
+  Local Definition bound_inj
+    : nat_map (bound_image_var L sigma) (bound_image_var L sigma') :=
+    inj_from_smaller decV
+                     (biv_card_list sigma finsigH)
+                     (biv_card_list sigma' finsig'H) cardleH id.
+
+  Local Lemma bound_inj_is_inj : inj_nat_map bound_inj.
+  Proof.
+    eauto using inj_from_smaller_is_inj.
+  Qed.
+
+  Definition split_rho : V -> V :=
+    split_map _ _ _ dec_sigma_fv vrho (fun x => nm_bot bound_inj (proj1_sig x)).
+
+  Lemma split_rho_inj v v' : split_rho v = split_rho v' -> v = v'.
+  Proof.
+    revert v v'; apply inj_split.
+    - eauto using vrho_injective.
+    - intros x x'.
+      assert (bound_image_var _ _ x = proj1_sig x) as projH; auto.
+      assert (bound_image_var _ _ x' = proj1_sig x') as projH'; auto.
+      rewrite <- projH, <- projH'.
+      apply bound_inj_is_inj.
+    - intros x x'.
+      assert (bound_image_var _ _ x' = proj1_sig x') as projH'; auto.
+      rewrite <- projH', <- nat_map_nat; clear projH'.
+      unfold bound_image_var.
+      intro eqH.
+      apply (proj2_sig (nm_top bound_inj x')).
+      unfold bound_image_var; rewrite <- eqH.
+      apply vrho_is_fv_for_sigma'.
+  Qed.
+
+  Lemma split_rho_on_free v (freeH : is_sigma_fv v)
+    : split_rho v = vrho (exist _ v freeH).
+  Proof.
+    unfold split_rho, split_map.
+    destruct dec_sigma_fv; [ apply vrho_irrel | contradiction ].
+  Qed.
+
+  Lemma split_rho_sigma v
+    : comp_subst L (var_subst_subst L split_rho) sigma v = sigma' v.
+  Proof.
+    rewrite sigma'H.
+    revert v; apply comp_subst_determined_by_fvs; intro v.
+    unfold var_subst_subst, Basics.compose, split_rho, split_map.
+    destruct dec_sigma_fv; [ auto using vrho_correct | contradiction ].
+  Qed.
+
+  Definition bound_inj_bot (x : sig is_sigma_bv) : V :=
+    nm_bot bound_inj (proj1_sig x).
+
+  Lemma bound_inj_bot_irrel v bvH bvH'
+    : bound_inj_bot (exist _ v bvH) = bound_inj_bot (exist _ v bvH').
+  Proof.
+    auto.
+  Qed.
+
+  Definition bound_inj_nm_top (x : bound_in_image L sigma)
+    : option (mod_dom bv_proj bound_inj_bot) :=
+    match decV (bound_inj_bot x) (proj1_sig x) with
+    | left eqH => None
+    | right neH => Some (exist _ x neH)
+    end.
+
+  Definition bound_inj_nm_bot (v : V) : option V :=
+    match dec_sigma_fv v with
+    | left fvH => None
+    | right bdH =>
+      match decV (bound_inj_bot (exist _ v bdH)) v with
+      | left eqH => None
+      | right neH => Some v
+      end
+    end.
+
+  Lemma bound_inj_finite
+    : FiniteProj (fun (x : mod_dom bv_proj bound_inj_bot) =>
+                    (bv_proj (md_elt x))).
+  Proof.
+    destruct (proj2_sig (biv_card_list sigma finsigH)) as [ _ fullH ].
+    apply (finite_surj_option (fun x => bv_proj (md_elt x))
+                              bound_inj_nm_top bound_inj_nm_bot
+                              (exist _ (proj1_sig (biv_card_list sigma finsigH))
+                                     fullH)).
+    - unfold bound_inj_nm_top, bound_inj_nm_bot.
+      intro x; destruct x as [ v bdH ]; simpl.
+      destruct (dec_sigma_fv v) as [ | bdH' ]; [ contradiction | ].
+      rewrite (bound_inj_bot_irrel v bdH' bdH); clear bdH'.
+      destruct (decV (bound_inj_bot (exist _ v bdH)) v) as [ eqH | neH ];
+        simpl;
+        destruct (decV (bound_inj_bot (exist is_sigma_bv v bdH)) v);
+        tauto.
+    - intro d; destruct d as [ x neH ]; exists x.
+      destruct x as [ v bdH ]; simpl.
+      unfold bound_inj_nm_bot.
+      destruct (dec_sigma_fv v) as [ | bdH' ]; [ contradiction | ].
+      rewrite (bound_inj_bot_irrel v bdH' bdH); clear bdH'.
+      destruct (decV (bound_inj_bot (exist is_sigma_bv v bdH)) v);
+        [ contradiction | auto ].
+  Qed.
+
+  Lemma var_subst_split_rho
+    : var_subst split_rho.
+  Proof.
+    apply (fin_split V V is_sigma_fv);
+      auto using vrho_irrel, vrho_finite, bound_inj_finite.
+  Qed.
+
+  Definition split_rho_inv : V -> V :=
+    inj_subst_inv var_subst_split_rho split_rho_inj decV.
+
+  Lemma split_rho_inv_sigma' v
+    : comp_subst L (var_subst_subst L split_rho_inv) sigma' v = sigma v.
+  Proof.
+    unfold comp_subst;
+      rewrite sigma'H;
+      fold (comp_subst L (var_subst_subst L split_rho_inv)
+                       (comp_subst L rho sigma) v).
+    rewrite comp_subst_assoc.
+    rewrite <- (comp_subst_idl _ (sigma := sigma)).
+    apply (comp_subst_determined_by_fvs); clear v; intros v fvH.
+    unfold comp_subst.
+    assert (rho v = varTerm L (split_rho v)) as rhoH.
+    - rewrite (split_rho_on_free _ fvH), vrho_correct; auto.
+    - rewrite rhoH; simpl; unfold var_subst_subst, Basics.compose; apply f_equal.
+      destruct (ext_inverse_inj_subst var_subst_split_rho split_rho_inj decV).
+      auto.
+  Qed.
+End sequiv_means_perm_lt.
+Section sequiv_means_perm.
+  Variable L : lType.
+  Notation V := (Term.V L).
+
+  Variables sigma sigma' : Subst L.
+  Hypothesis finsigH : fin_subst L sigma.
+  Hypothesis finsig'H : fin_subst L sigma'.
+  Variables rho rho' : Subst L.
+  Hypothesis sigma'H : forall v, sigma' v = comp_subst L rho sigma v.
+  Hypothesis sigmaH : forall v, sigma v = comp_subst L rho' sigma' v.
+  Hypothesis finrhoH : fin_subst L rho.
+  Hypothesis finrho'H : fin_subst L rho'.
+  Hypothesis decV : forall v v' : V, {v = v'} + {v <> v'}.
+
+  Local Definition tau : V -> V :=
+    match le_ge_dec (biv_card L decV sigma finsigH) (biv_card L decV sigma' finsig'H) with
+    | left leH => split_rho L sigma sigma' rho rho'
+                            sigma'H sigmaH finsigH finsig'H decV leH
+    | right geH => split_rho_inv L sigma' sigma rho' rho sigmaH
+                                 sigma'H finsig'H finsigH finrho'H decV geH
+    end.
+
+  Lemma tau_sigma v
+    : comp_subst L (var_subst_subst L tau) sigma v = sigma' v.
+  Proof.
+    unfold tau; destruct (le_ge_dec _ _);
+      auto using split_rho_sigma, split_rho_inv_sigma'.
+  Qed.
+
+  Local Definition tau' : V -> V :=
+    match le_ge_dec (biv_card L decV sigma finsigH) (biv_card L decV sigma' finsig'H) with
+    | left leH => split_rho_inv L sigma sigma' rho rho' sigma'H
+                                sigmaH finsigH finsig'H finrhoH decV leH
+    | right geH => split_rho L sigma' sigma rho' rho
+                             sigmaH sigma'H finsig'H finsigH decV geH
+    end.
+
+  Lemma tau'_sigma' v
+    : comp_subst L (var_subst_subst L tau') sigma' v = sigma v.
+  Proof.
+    unfold tau'; destruct (le_ge_dec _ _);
+      auto using split_rho_sigma, split_rho_inv_sigma'.
+  Qed.
+
+  Lemma ext_inverse_tau : ext_inverse tau tau'.
+  Proof.
+    unfold tau, tau'; destruct (le_ge_dec _ _);
+      [ | apply ext_inverse_sym ];
+      apply ext_inverse_inj_subst.
+  Qed.
+
+  Lemma var_subst_tau : var_subst tau.
+  Proof.
+    unfold tau; destruct (le_ge_dec _ _).
+    - auto using var_subst_split_rho, finrhoH.
+    - apply var_subst_inj_subst_inv.
+  Qed.
+
+  Lemma var_subst_tau' : var_subst tau'.
+  Proof.
+    unfold tau'; destruct (le_ge_dec _ _).
+    - apply var_subst_inj_subst_inv.
+    - auto using var_subst_split_rho, finrhoH.
   Qed.
 
 End sequiv_means_perm.
